17-03
18:13

Protocol/BlockchainNew.thy
@@ -1,20 +1,31 @@
 theory BlockchainNew
   imports Main "HOL-Library.Tree"
 begin
+type_synonym Transactions = nat
 
-datatype Hash = H nat nat 
+type_synonym Party = nat
+type_synonym Slot = nat
+
+(*type_synonym Hash = "nat list"*)
+datatype Hash = H nat nat
+definition "Slotzero = 0"
+type_synonym Delay = nat
+type_synonym Parties = "Party list"
+ 
+fun Winner :: "Party \<Rightarrow> Slot \<Rightarrow> bool" where
+"Winner P S = (if P = S then True else False)"
+
+
+(*"Hash option"*)
 record Block =
-  sl :: nat
-  txs :: nat
+  sl :: Slot
+  txs :: Transactions
   pred :: Hash
-  bid :: nat
+  bid :: Party
 
 type_synonym Chain = "Block list"
 type_synonym Chains = "Chain list"
 type_synonym BlockPool = "Block list"
-
-fun Winner :: "nat \<Rightarrow> nat \<Rightarrow> bool" where
-"Winner P S = (if P = S then True else False)"
 
 fun HashCompare :: "Hash \<Rightarrow> Block \<Rightarrow> bool" where
 "HashCompare (H a b) bl1 = (if ((a = sl bl1) \<and> (b = bid bl1)) then True else False)"
@@ -22,164 +33,176 @@ fun HashCompare :: "Hash \<Rightarrow> Block \<Rightarrow> bool" where
 fun HashB :: "Block \<Rightarrow> Block \<Rightarrow> bool" where
 "HashB bl1 bl2 = HashCompare (pred bl2) bl1"
 
-
 definition "GenBlock = \<lparr>sl = 0, txs = 0, pred = H 0 0 ,bid = 0\<rparr>"
 definition "Block1 = \<lparr>sl = 1, txs =1, pred = H 0 0, bid = 1\<rparr>"
 
 value "HashB GenBlock Block1"
 
 fun valid_blocks ::"Block \<Rightarrow> Block \<Rightarrow> bool" where
-"valid_blocks b1 b2 = (Winner (sl b1) (bid b1) \<and> HashB b2 b1 \<and> (sl b2 < sl b1)) "
-value "valid_blocks Block1 GenBlock"
-fun valid_chain :: "Chain \<Rightarrow> bool" where
-"valid_chain [] = False"|
-"valid_chain [b1] = (if b1 = GenBlock then True else False)"|
-"valid_chain (b1#b2#c) = (if b1 \<noteq> b2\<and> valid_blocks b1 b2 \<and> (b1 \<noteq> GenBlock) then valid_chain (b2#c) else False)"
+"valid_blocks b1 b2 = (HashB b2 b1 \<and> (sl b2 \<le> sl b1)) "
 
-datatype T = Leaf | GenesisNode Block T T | Node Block T T   
-fun allBlocks2 :: "T \<Rightarrow> BlockPool" where
-"allBlocks2 (Node m l r) = allBlocks2 l@allBlocks2 r @[m]"|
-"allBlocks2 (GenesisNode m l r) = [] " |
-"allBlocks2 Leaf = []"
+
+value "valid_blocks Block1 GenBlock"
+value "a#b#[c,d]"
+
+(*checking for b's being a node only and a /genesis node at the end of the list missing*)
+fun valid_chain :: "Chain \<Rightarrow> bool" where
+"valid_chain [] = True"|
+"valid_chain [b1] = (if b1 = GenBlock then True else False)"|
+"valid_chain (b1#b2#c) = (if valid_blocks b1 b2 \<and> (b1 \<noteq> GenBlock) then valid_chain (b2#c) else False)"
+
+
+value "valid_chain [\<lparr>sl = 2, txs = 2, pred = H 1 1, bid = 2\<rparr>, \<lparr>sl = 1, txs = 1, pred = H 0 0, bid = 1\<rparr>, \<lparr>sl = 0, txs = 0, pred = H 0 0, bid = 0\<rparr>]"
+value "HashB  \<lparr>sl = 1, txs = 1, pred = H 0 0, bid = 1\<rparr> \<lparr>sl = 2, txs = 1, pred = H 1 1, bid = 2\<rparr>"
+
+datatype T = Leaf | Node Block T T 
+datatype GenT = GenesisNode Block T T
+
 fun allBlocks :: "T \<Rightarrow> BlockPool" where
-"allBlocks (Node m l r) = []"|
-"allBlocks (GenesisNode m l r) = allBlocks2 l@allBlocks2 r @[m] " |
+"allBlocks (Node m l r) = allBlocks l@allBlocks r @[m]"|
 "allBlocks Leaf = []"
 
+fun allBlocksGen :: "GenT \<Rightarrow> BlockPool" where
+"allBlocksGen (GenesisNode m l r) = allBlocks l@allBlocks r @[m] "
 
 fun allBlocksAppend :: "Block \<Rightarrow>BlockPool list\<Rightarrow> BlockPool list" where
 "allBlocksAppend Bl BlP = (map (\<lambda> bl. bl @ [Bl]) BlP)"
 
+fun allBlocks2 :: "T \<Rightarrow> BlockPool list" where
+"allBlocks2 (Node m l r) = allBlocksAppend m (allBlocks2 l) @allBlocksAppend m (allBlocks2 r)"|
+"allBlocks2 Leaf = [[]]"
 
-fun allBlocks' :: "T \<Rightarrow> BlockPool list" where
-"allBlocks' (Node m l r) = allBlocksAppend m (allBlocks' l) @allBlocksAppend m (allBlocks' r)"|
-"allBlocks' (GenesisNode m l r) = allBlocksAppend m (allBlocks' l) @allBlocksAppend m (allBlocks' r)"|
-"allBlocks' Leaf = [[]]"
+fun allBlocks' :: "GenT \<Rightarrow> BlockPool list" where
+"allBlocks' (GenesisNode m l r) = allBlocksAppend m (allBlocks2 l) @allBlocksAppend m (allBlocks2 r)"
+
+
 
 definition "tree0 = GenesisNode GenBlock Leaf Leaf"
-
-lemma initialTree : "allBlocks tree0 = [GenBlock]" 
+definition "exampleTree = (GenesisNode GenBlock (Node Block1 Leaf Leaf) (Node Block1 Leaf Leaf))"
+lemma initialTree : "allBlocksGen tree0 = [GenBlock]" 
   by (simp add: GenBlock_def tree0_def)
+value "set(allBlocksGen exampleTree) = {\<lparr>sl = 1, txs = 1, pred = H 0 0, bid = 1\<rparr>,
+  \<lparr>sl = 0, txs = 0, pred = H 0 0, bid = 0\<rparr>}"
+value "allBlocks' exampleTree"
+
 
 fun extendTree :: "T \<Rightarrow> Block \<Rightarrow> T" where
-"extendTree (GenesisNode Bl1 Leaf Leaf) Bl2 = (if (valid_blocks Bl2 Bl1) then (GenesisNode Bl1 (Node Bl2 Leaf Leaf) Leaf) else (GenesisNode Bl1 Leaf Leaf)) "|
 "extendTree (Node Bl1 Leaf Leaf) Bl2 =  (if valid_blocks Bl2 Bl1 then (Node Bl1 (Node Bl2 Leaf Leaf) Leaf) else (Node Bl1 Leaf Leaf)) "|
-"extendTree (GenesisNode Bl1 t1 Leaf) Bl2 =  (if valid_blocks Bl2 Bl1  then (GenesisNode Bl1 t1 (Node Bl2 Leaf Leaf)) else (GenesisNode Bl1 (extendTree t1 Bl2) Leaf))"|
 "extendTree (Node Bl1 t1 Leaf) Bl2 =  (if valid_blocks Bl2 Bl1 then (Node Bl1 t1 (Node Bl2 Leaf Leaf)) else (Node Bl1 (extendTree t1 Bl2) Leaf))"|
-"extendTree (GenesisNode Bl1 t1 t2) Bl2 = (GenesisNode Bl1 (extendTree t1 Bl2) (extendTree t2 Bl2))"|
+"extendTree (Node Bl1 Leaf t1) Bl2 =  (if valid_blocks Bl2 Bl1 then (Node Bl1 (Node Bl2 Leaf Leaf) t1) else (Node Bl1 Leaf (extendTree t1 Bl2)))"|
 "extendTree (Node Bl1 t1 t2) Bl2 =(Node Bl1 (extendTree t1 Bl2) (extendTree t2 Bl2))"|
 "extendTree Leaf Bl2 = Leaf"
 
+fun extendTreeGen :: "GenT \<Rightarrow> Block \<Rightarrow> GenT" where
+"extendTreeGen (GenesisNode Bl1 Leaf Leaf) Bl2 = (if valid_blocks Bl2 Bl1 then (GenesisNode Bl1 (Node Bl2 Leaf Leaf) Leaf) else (GenesisNode Bl1 Leaf Leaf)) "|
+"extendTreeGen (GenesisNode Bl1 t1 Leaf) Bl2 =  (if valid_blocks Bl2 Bl1  then (GenesisNode Bl1 t1 (Node Bl2 Leaf Leaf)) else (GenesisNode Bl1 (extendTree t1 Bl2) Leaf))"|
+"extendTreeGen (GenesisNode Bl1 Leaf t1) Bl2 =  (if valid_blocks Bl2 Bl1 then (GenesisNode Bl1 (Node Bl2 Leaf Leaf) t1) else (GenesisNode Bl1 Leaf (extendTree t1 Bl2)))"|
+"extendTreeGen (GenesisNode Bl1 t1 t2) Bl2 = (GenesisNode Bl1 (extendTree t1 Bl2) (extendTree t2 Bl2))"
+lemma "extendTree Leaf B = Leaf"
+  by simp
+
 definition valid_t where
 "valid_t t = (\<forall>c\<in>set(allBlocks' t).valid_chain c)"
-value "valid_t (GenesisNode \<lparr>sl = 0, txs = 0, pred = H 0 0, bid = 0\<rparr> T.Leaf
-       (GenesisNode \<lparr>sl = 0, txs = 0, pred = H 0 0, bid = 0\<rparr> T.Leaf T.Leaf))"
-lemma "extendTree Leaf B = Leaf" 
-  by simp
-value "extendTree (GenesisNode GenBlock Leaf Leaf) \<lparr>sl = 1, txs = 0, pred = H 0 0, bid = 1\<rparr>"
-fun root2 :: "T \<Rightarrow> bool" where
-"root2 Leaf = True"|
-"root2 (Node Bl l r) = (if Bl \<noteq> GenBlock then True \<and> root2 l \<and> root2 r  else False)"|
-"root2 (GenesisNode _ _ _) = False"
 
-fun root :: "T \<Rightarrow> bool" where
-"root (GenesisNode Bl l r) = (if Bl = GenBlock then True \<and> root2 l  \<and> root2 r else False)"|
-"root (Node _ _ _) = False"|
-"root Leaf = False"
-
-lemma AllExtend : "extendTree   t b \<noteq> t \<and> (valid_t t) \<and> root t \<Longrightarrow> set (allBlocks (extendTree t b)) =set ([b]@ allBlocks t)"
+lemma AllExtend : "(extendTreeGen t b) \<noteq> t  \<Longrightarrow> set (allBlocksGen (extendTreeGen t b)) =set ([b]@ allBlocksGen t)"
 proof(induction t)
-  case Leaf
-  then show ?case by simp
-next
-  case (GenesisNode x1 t1 t2) note ABC=this
-  then show ?case proof (cases "t1") 
-    case Leaf note t1Leaf=this
-    then show ?thesis proof (cases "t2")
+  case (GenesisNode x1a x2a x3a) note Gen = this
+  then show ?case proof (cases "x2a")
+    case Leaf note x2aLeaf = this
+    then show ?thesis proof (cases "x3a")
       case Leaf
-      then show ?thesis using ABC t1Leaf
-        by auto   
-    next
-      case (GenesisNode x21 x22 x23)
-      then show ?thesis using ABC t1Leaf
-        by (metis root.simps(1) root2.simps(3))
-    next
-      case (Node x31 x32 x33)
-      then show ?thesis using ABC t1Leaf
-        try
-    qed
-  next
-    case (GenesisNode x21 x22 x23) note GenNode1=this
-    then show ?thesis proof(cases "t2")
-      case Leaf
-      then show ?thesis using ABC GenNode1 
-        by (metis root.simps(1) root2.simps(3))
-    next
-      case (GenesisNode x21 x22 x23)
-      then show ?thesis using ABC GenNode1 
-        try
-    next
-      case (Node x31 x32 x33)
-      then show ?thesis using ABC GenNode1 
-        try
-    qed
-  next
-    case (Node x31 x32 x33) note Node1=this
-    then show ?thesis proof(cases "t2" )
-      case Leaf
-      then show ?thesis using ABC Node1 by auto
-    next
-      case (GenesisNode x21 x22 x23)
-      then show ?thesis using ABC Node1 by fastforce
-    next
-      case (Node x31 x32 x33)
-      then show ?thesis using ABC Node1 by fastforce
-    qed 
-  qed 
-next
-  case (Node x1 t1 t2) note NodeA = this
-  then show ?case proof(cases "t1")
-    case Leaf note t2Leaf=this
-    then show ?thesis proof(cases "t2")
-      case Leaf
-      then show ?thesis using NodeA t2Leaf
+      then show ?thesis using Gen x2aLeaf 
         by auto
     next
-      case (GenesisNode x21 x22 x23)
-      then show ?thesis  using NodeA t2Leaf
-        by auto
-    next
-      case (Node x31 x32 x33)
-      then show ?thesis  using NodeA t2Leaf
-        by auto
+      case (Node x21 x22 x23)
+      then show ?thesis using Gen x2aLeaf by auto
     qed
   next
-    case (GenesisNode x21 x22 x23) note t2GenNodeA = this
-    then show ?thesis proof(cases "t2")
+    case (Node x21 x22 x23) note x2aNode = this
+    then show ?thesis proof (cases "x3a")
       case Leaf
-      then show ?thesis using NodeA t2GenNodeA
-        by auto
+      then show ?thesis using Gen x2aNode sorry
     next
-      case (GenesisNode x21 x22 x23)
-      then show ?thesis  using NodeA t2GenNodeA  by fastforce
-    next
-      case (Node x31 x32 x33)
-      then show ?thesis using NodeA t2GenNodeA  by fastforce
+      case (Node x21 x22 x23)
+      then show ?thesis using Gen x2aNode sorry
     qed
-  next
-    case (Node x31 x32 x33) note t2NodeA = this
-    then show ?thesis proof(cases "t2")
-      case Leaf
-      then show ?thesis using NodeA t2NodeA by auto
-    next
-      case (GenesisNode x21 x22 x23)
-      then show ?thesis using NodeA t2NodeA 
-        by fastforce
-    next
-      case (Node x31 x32 x33)
-      then show ?thesis using NodeA t2NodeA by fastforce
-    qed
-  qed 
+  qed
 qed
 
 
+value "extendTreeGen (GenesisNode GenBlock Leaf Leaf) Block1 "
+value "extendTreeGen (GenesisNode GenBlock (Node \<lparr>sl = 1, txs = 1, pred = H 0 0, bid = 1\<rparr> Leaf Leaf) (Node \<lparr>sl = 1, txs = 1, pred = H 0 0, bid = 2\<rparr> Leaf Leaf)) \<lparr>sl = 0, txs = 0, pred =H 1 2, bid = 1\<rparr> "
+value "extendTreeGen (GenesisNode GenBlock (Node Block1 Leaf Leaf) Leaf) \<lparr>sl = 1, txs = 1, pred = H 1 2, bid = 1\<rparr> "
+value "extendTreeGen (GenesisNode GenBlock Leaf Leaf) Block1 "
+
+fun best_c :: "nat \<Rightarrow> Block list list \<Rightarrow> (Block list \<times> nat \<times> bool) option"where 
+"best_c slot list = (let list' = map (\<lambda> l. (l,sl (hd l), valid_chain l)) list in find (\<lambda> (c,s,v).v\<and>(s\<le>slot)) list')"
+
+definition get_first :: \<open>(Block list \<times> nat \<times> bool) option \<Rightarrow>Block list\<close> where
+\<open>get_first a = (case a of None \<Rightarrow> [] | Some a \<Rightarrow> fst a)\<close>
+
+lemma best_c_none : "best_c n [] = None"
+  by(simp)
+
+lemma find_in : \<open>find p ls = Some l\<Longrightarrow> l\<in> set(ls)\<close>
+proof(induction ls)
+  case Nil
+  then show ?case by simp
+next
+  case (Cons a ls)
+  then show ?case
+    by (metis find_Some_iff nth_mem)
+qed
+
+lemma best_c_in : "best_c n bl \<noteq> None \<Longrightarrow>  get_first(best_c n bl) \<in> set(bl)"
+  apply(simp add:get_first_def find_in)
+proof(induction bl)
+  case Nil
+  then show ?case
+    by simp 
+next
+  case (Cons a bl)
+  then show ?case
+    by auto
+qed
+
+fun best_chain :: "Slot \<Rightarrow> GenT \<Rightarrow> Block list" where
+"best_chain 0 (GenesisNode x _ _) = (if x = GenBlock then [GenBlock]else [])"|
+"best_chain s T = get_first ( best_c s (allBlocks' T))"
+
+value "best_c (3::nat) (allBlocks' ((GenesisNode GenBlock (Node \<lparr>sl = 1, txs = 1, pred = H 0 0, bid = 1\<rparr>  Leaf Leaf)
+ (Node \<lparr>sl = 1, txs = 1, pred = H 0 0, bid = 2\<rparr> Leaf Leaf))))"
+value "allBlocks' ((GenesisNode GenBlock (Node \<lparr>sl = 1, txs = 1, pred = H 0 0, bid = 1\<rparr> (Node \<lparr>sl = 1, txs = 1, pred = H 1 1, bid = 1\<rparr> Leaf Leaf) Leaf)
+ (Node \<lparr>sl = 1, txs = 1, pred = H 1 1, bid = 1\<rparr> Leaf Leaf)))"
+
+value "valid_chain (best_chain 2 (GenesisNode GenBlock (Node \<lparr>sl = 1, txs = 1, pred = H 0 0, bid = 1\<rparr> (Node \<lparr>sl = 1, txs = 1, pred = H 1 1, bid = 1\<rparr> (Node \<lparr>sl = 2, txs = 2, pred = H 1 1, bid = 2\<rparr> Leaf Leaf) Leaf) Leaf)
+ (Node \<lparr>sl = 1, txs = 1, pred = H 1 1, bid = 1\<rparr> Leaf Leaf)))"
+
+value "best_chain 1 (GenesisNode \<lparr>sl = 0, txs = 0, pred = H 0 0, bid = 1\<rparr> Leaf Leaf)"
+value "allBlocks'  (GenesisNode \<lparr>sl = 0, txs = 0, pred = H 0 0, bid = 1\<rparr> Leaf Leaf)"
+
+lemma best_valid :"\<forall>s. valid_t t \<and> (allBlocks' t \<noteq>[[]]) \<Longrightarrow> valid_chain (best_chain s t)"
+  proof(induction t)
+    case (GenesisNode x1a x2a x3a) note Gen = this
+    then show ?case proof (cases "x2a")
+      case Leaf note Leafa = this
+      then show ?thesis proof (cases "x3a")
+        case Leaf
+        then show ?thesis using Leafa Gen try
+      next
+        case (Node x21 x22 x23)
+        then show ?thesis using Leafa Gen
+      qed
+    next
+      case (Node x21 x22 x23)
+      then show ?thesis proof (cases "x3a")
+        case Leaf
+        then show ?thesis sorry
+      next
+        case (Node x21 x22 x23)
+        then show ?thesis sorry
+      qed
+    qed
+  qed
+
+  
