Protocol/BlockchainNew.thy~
@@ -1,0 +1,185 @@
+theory BlockchainNew
+  imports Main "HOL-Library.Tree"
+begin
+
+datatype Hash = H nat nat 
+record Block =
+  sl :: nat
+  txs :: nat
+  pred :: Hash
+  bid :: nat
+
+type_synonym Chain = "Block list"
+type_synonym Chains = "Chain list"
+type_synonym BlockPool = "Block list"
+
+fun Winner :: "nat \<Rightarrow> nat \<Rightarrow> bool" where
+"Winner P S = (if P = S then True else False)"
+
+fun HashCompare :: "Hash \<Rightarrow> Block \<Rightarrow> bool" where
+"HashCompare (H a b) bl1 = (if ((a = sl bl1) \<and> (b = bid bl1)) then True else False)"
+
+fun HashB :: "Block \<Rightarrow> Block \<Rightarrow> bool" where
+"HashB bl1 bl2 = HashCompare (pred bl2) bl1"
+
+
+definition "GenBlock = \<lparr>sl = 0, txs = 0, pred = H 0 0 ,bid = 0\<rparr>"
+definition "Block1 = \<lparr>sl = 1, txs =1, pred = H 0 0, bid = 1\<rparr>"
+
+value "HashB GenBlock Block1"
+
+fun valid_blocks ::"Block \<Rightarrow> Block \<Rightarrow> bool" where
+"valid_blocks b1 b2 = (Winner (sl b1) (bid b1) \<and> HashB b2 b1 \<and> (sl b2 < sl b1)) "
+value "valid_blocks Block1 GenBlock"
+fun valid_chain :: "Chain \<Rightarrow> bool" where
+"valid_chain [] = False"|
+"valid_chain [b1] = (if b1 = GenBlock then True else False)"|
+"valid_chain (b1#b2#c) = (if b1 \<noteq> b2\<and> valid_blocks b1 b2 \<and> (b1 \<noteq> GenBlock) then valid_chain (b2#c) else False)"
+
+datatype T = Leaf | GenesisNode Block T T | Node Block T T   
+fun allBlocks2 :: "T \<Rightarrow> BlockPool" where
+"allBlocks2 (Node m l r) = allBlocks2 l@allBlocks2 r @[m]"|
+"allBlocks2 (GenesisNode m l r) = [] " |
+"allBlocks2 Leaf = []"
+fun allBlocks :: "T \<Rightarrow> BlockPool" where
+"allBlocks (Node m l r) = []"|
+"allBlocks (GenesisNode m l r) = allBlocks2 l@allBlocks2 r @[m] " |
+"allBlocks Leaf = []"
+
+
+fun allBlocksAppend :: "Block \<Rightarrow>BlockPool list\<Rightarrow> BlockPool list" where
+"allBlocksAppend Bl BlP = (map (\<lambda> bl. bl @ [Bl]) BlP)"
+
+
+fun allBlocks' :: "T \<Rightarrow> BlockPool list" where
+"allBlocks' (Node m l r) = allBlocksAppend m (allBlocks' l) @allBlocksAppend m (allBlocks' r)"|
+"allBlocks' (GenesisNode m l r) = allBlocksAppend m (allBlocks' l) @allBlocksAppend m (allBlocks' r)"|
+"allBlocks' Leaf = [[]]"
+
+definition "tree0 = GenesisNode GenBlock Leaf Leaf"
+
+lemma initialTree : "allBlocks tree0 = [GenBlock]" 
+  by (simp add: GenBlock_def tree0_def)
+
+fun extendTree :: "T \<Rightarrow> Block \<Rightarrow> T" where
+"extendTree (GenesisNode Bl1 Leaf Leaf) Bl2 = (if (valid_blocks Bl2 Bl1) then (GenesisNode Bl1 (Node Bl2 Leaf Leaf) Leaf) else (GenesisNode Bl1 Leaf Leaf)) "|
+"extendTree (Node Bl1 Leaf Leaf) Bl2 =  (if valid_blocks Bl2 Bl1 then (Node Bl1 (Node Bl2 Leaf Leaf) Leaf) else (Node Bl1 Leaf Leaf)) "|
+"extendTree (GenesisNode Bl1 t1 Leaf) Bl2 =  (if valid_blocks Bl2 Bl1  then (GenesisNode Bl1 t1 (Node Bl2 Leaf Leaf)) else (GenesisNode Bl1 (extendTree t1 Bl2) Leaf))"|
+"extendTree (Node Bl1 t1 Leaf) Bl2 =  (if valid_blocks Bl2 Bl1 then (Node Bl1 t1 (Node Bl2 Leaf Leaf)) else (Node Bl1 (extendTree t1 Bl2) Leaf))"|
+"extendTree (GenesisNode Bl1 t1 t2) Bl2 = (GenesisNode Bl1 (extendTree t1 Bl2) (extendTree t2 Bl2))"|
+"extendTree (Node Bl1 t1 t2) Bl2 =(Node Bl1 (extendTree t1 Bl2) (extendTree t2 Bl2))"|
+"extendTree Leaf Bl2 = Leaf"
+
+definition valid_t where
+"valid_t t = (\<forall>c\<in>set(allBlocks' t).valid_chain c)"
+value "valid_t (GenesisNode \<lparr>sl = 0, txs = 0, pred = H 0 0, bid = 0\<rparr> T.Leaf
+       (GenesisNode \<lparr>sl = 0, txs = 0, pred = H 0 0, bid = 0\<rparr> T.Leaf T.Leaf))"
+lemma "extendTree Leaf B = Leaf" 
+  by simp
+value "extendTree (GenesisNode GenBlock Leaf Leaf) \<lparr>sl = 1, txs = 0, pred = H 0 0, bid = 1\<rparr>"
+fun root2 :: "T \<Rightarrow> bool" where
+"root2 Leaf = True"|
+"root2 (Node Bl l r) = (if Bl \<noteq> GenBlock then True \<and> root2 l \<and> root2 r  else False)"|
+"root2 (GenesisNode _ _ _) = False"
+
+fun root :: "T \<Rightarrow> bool" where
+"root (GenesisNode Bl l r) = (if Bl = GenBlock then True \<and> root2 l  \<and> root2 r else False)"|
+"root (Node _ _ _) = False"|
+"root Leaf = False"
+
+lemma AllExtend : "extendTree   t b \<noteq> t \<and> (valid_t t) \<and> root t \<Longrightarrow> set (allBlocks (extendTree t b)) =set ([b]@ allBlocks t)"
+proof(induction t)
+  case Leaf
+  then show ?case by simp
+next
+  case (GenesisNode x1 t1 t2) note ABC=this
+  then show ?case proof (cases "t1") 
+    case Leaf note t1Leaf=this
+    then show ?thesis proof (cases "t2")
+      case Leaf
+      then show ?thesis using ABC t1Leaf
+        by auto   
+    next
+      case (GenesisNode x21 x22 x23)
+      then show ?thesis using ABC t1Leaf
+        by (metis root.simps(1) root2.simps(3))
+    next
+      case (Node x31 x32 x33)
+      then show ?thesis using ABC t1Leaf
+        try
+    qed
+  next
+    case (GenesisNode x21 x22 x23) note GenNode1=this
+    then show ?thesis proof(cases "t2")
+      case Leaf
+      then show ?thesis using ABC GenNode1 
+        by (metis root.simps(1) root2.simps(3))
+    next
+      case (GenesisNode x21 x22 x23)
+      then show ?thesis using ABC GenNode1 
+        try
+    next
+      case (Node x31 x32 x33)
+      then show ?thesis using ABC GenNode1 
+        try
+    qed
+  next
+    case (Node x31 x32 x33) note Node1=this
+    then show ?thesis proof(cases "t2" )
+      case Leaf
+      then show ?thesis using ABC Node1 by auto
+    next
+      case (GenesisNode x21 x22 x23)
+      then show ?thesis using ABC Node1 by fastforce
+    next
+      case (Node x31 x32 x33)
+      then show ?thesis using ABC Node1 by fastforce
+    qed 
+  qed 
+next
+  case (Node x1 t1 t2) note NodeA = this
+  then show ?case proof(cases "t1")
+    case Leaf note t2Leaf=this
+    then show ?thesis proof(cases "t2")
+      case Leaf
+      then show ?thesis using NodeA t2Leaf
+        by auto
+    next
+      case (GenesisNode x21 x22 x23)
+      then show ?thesis  using NodeA t2Leaf
+        by auto
+    next
+      case (Node x31 x32 x33)
+      then show ?thesis  using NodeA t2Leaf
+        by auto
+    qed
+  next
+    case (GenesisNode x21 x22 x23) note t2GenNodeA = this
+    then show ?thesis proof(cases "t2")
+      case Leaf
+      then show ?thesis using NodeA t2GenNodeA
+        by auto
+    next
+      case (GenesisNode x21 x22 x23)
+      then show ?thesis  using NodeA t2GenNodeA  by fastforce
+    next
+      case (Node x31 x32 x33)
+      then show ?thesis using NodeA t2GenNodeA  by fastforce
+    qed
+  next
+    case (Node x31 x32 x33) note t2NodeA = this
+    then show ?thesis proof(cases "t2")
+      case Leaf
+      then show ?thesis using NodeA t2NodeA by auto
+    next
+      case (GenesisNode x21 x22 x23)
+      then show ?thesis using NodeA t2NodeA 
+        by fastforce
+    next
+      case (Node x31 x32 x33)
+      then show ?thesis using NodeA t2NodeA by fastforce
+    qed
+  qed 
+qed
+
+
